code/rocq/elpi2.v
@@ -1,0 +1,1098 @@
+From mathcomp Require Import all_ssreflect.
+From det Require Import lang valid_state.
+From elpi.apps Require Import derive derive.std.
+From HB Require Import structures.
+
+Lemma ltn_leq_trans m n p :
+  m < n -> n <= p -> m < p.
+Proof.
+  move=> Hmn Hnp.
+  apply: leq_trans Hmn Hnp.
+Qed.
+
+Lemma add_succ {x}: x = x.+1 -> False.
+Proof. elim: x => // n H; inversion 1; auto. Qed.
+
+Lemma flatten_empty {T R : Type} {l: list T}:
+  @flatten R [seq [::] | _ <- l] = [::].
+Proof. elim: l => //. Qed.
+
+Lemma cats20 {T: Type} {X Y : list T}: X ++ Y = [::] -> X = [::] /\ Y = [::].
+Proof. by destruct X. Qed.
+
+Lemma size_list {T : Type} {l1 l2: list T}: l1 = l2 -> size l1 = size l2.
+Proof. move=>->//. Qed.
+
+Lemma cat_nil {T: Type} {l1 l2: list T}: l2 = l1 ++ l2 -> l1 = [::].
+Proof.
+  elim: l2 l1 => [|x xs IH] l1.
+    rewrite cats0//.
+  case: l1 => //y ys[<-].
+  rewrite (catA _ [::x])=>/IH.
+  case: ys => //.
+Qed.
+
+Lemma cons_false {T: Type} {x:T} {xs}: x :: xs = xs -> False.
+Proof. elim: xs x => //x xs IH y[_/IH]//. Qed.
+
+Lemma addSn_false {a b}: a = a + b.+1 -> False.
+Proof. elim: a b => // n H n1 []/H//. Qed.
+
+Lemma cat_same_tl {T : Type} {l1 l2 l3: list T}: l1 ++ l3 = l2 ++ l3 -> l1 = l2.
+Proof. 
+  elim: l1 l2 l3 => //.
+    move=>[]//x xs l3/=.
+    rewrite -cat_cons.
+    move=>/cat_nil//.
+  move=> x xs IH [|y ys]//l3.
+    move=>/=/esym; rewrite -cat_cons => /cat_nil//.
+  move=>[<-]/IH->//.
+Qed.
+
+Module Nur (U : Unif).
+
+  Module VS := valid_state(U).
+  Import VS RunP Run Language.
+  
+  (* The bool in the cut is to know if the cut is deep.
+     For expamle, in the state:
+      ((! \/ A) /\ !) \/ C
+    The first cut is deep, therefore its cut-to alternatives point to C
+    The second cut is superficial, therfore its cut to alternatives are empty
+  *)
+  Inductive G := 
+    | call : program -> Tm -> G
+    | cut : list (list G) -> G
+    .
+
+  Definition if_cut F g :=
+    match g with
+    | cut a => F a
+    | _ => true
+    end.
+
+  Definition apply_cut F g :=
+    match g with
+    | cut a => cut (F a) 
+    | _ => g
+    end.
+
+  derive G.
+  HB.instance Definition _ := hasDecEq.Build G G_eqb_OK.
+
+  Definition alt := (list G).
+
+  Definition a2g p A :=
+    match A with
+    | Cut => cut [::]
+    | Call t => call p t
+    end.
+
+  Definition a2gs p (b : Sigma * R) :=
+    map (a2g p) b.2.(premises).
+
+  Section add_ca.
+
+    Definition add_ca alts a := (*always:= adds always alts to cut *)
+      match a with
+      | cut a1 => cut (a1 ++ alts)
+      | call pr t => call pr t
+      end.
+
+    Lemma add_ca_empty {lA}:
+      map (add_ca [::]) lA = lA.
+    Proof.
+      rewrite /add_ca; elim: lA => //= x xs IH.
+      rewrite IH; case: x => // l; rewrite cats0//if_same//.
+    Qed.
+
+    Lemma map_add0_cas_empty {lA}:
+      map (map (add_ca [::])) lA  = lA.
+    Proof.
+      rewrite /add_ca; elim: lA => //= x xs ->.
+      f_equal; apply add_ca_empty.
+    Qed.
+  End add_ca.
+
+
+  Definition save_alt a gs b := map (add_ca a) b ++ gs.
+  Definition more_alt a bs gs := map (save_alt a gs) bs ++ a.
+
+  Inductive nur : Sigma -> list G ->  list alt -> Sigma -> list alt -> Prop :=
+  | StopE s a : nur s [::] a s a
+  | CutE s s1 a ca r gl : nur s gl ca s1 r -> nur s [:: cut ca & gl] a s1 r
+  | CallE p s s1 a b bs gl r t : 
+    F p t s = [:: b & bs ] -> 
+      nur s (save_alt a (a2gs p b) gl) (more_alt a (map (a2gs p) bs) gl) s1 r -> 
+        nur s [::call p t & gl] a s1 r
+  | FailE p s s1 t gl a al r : 
+    F p t s = [::] -> nur s a al s1 r -> nur s [::call p t & gl] (a :: al) s1 r.
+
+  Lemma nur_consistent {s G x xs1 xs2 s1 s2} :
+    nur s G x s1 xs1 -> nur s G x s2 xs2 -> xs1 = xs2 /\ s1 = s2.
+  Proof.
+    move=> H; elim: H xs2 s2 => //; clear.
+    - inversion 1 => //.
+    - move=> p s a ca r gl H IH xs2.
+      by inversion 1; subst; auto.
+    - move=> p s s1 a b bs gl r t H H1 IH xs2 s2 H2.
+      apply: IH.
+      inversion H2; subst; move: H9; rewrite H => //-[??]; subst.
+      apply: H10.
+    - move=> p1 s s1 t gl a al r H H1 IH xs2 s2 H2.
+      apply: IH.
+      inversion H2; subst => //.
+      congruence.
+  Qed.
+
+  Section t2l.
+
+    Inductive G' := 
+      | call' : program -> Tm -> G'
+      | cut' : bool -> list (list G') -> G'
+      .
+    derive G'.
+    HB.instance Definition _ := hasDecEq.Build G' G'_eqb_OK.
+
+
+    Definition apply_cut1 F g :=
+      match g with
+      | cut' b1 a => cut' b1 (F a) 
+      | _ => g
+      end.
+
+    Definition if_cut1 F g :=
+      match g with
+      | cut' b1 a => (F a) 
+      | _ => true
+      end.
+
+    Definition get_ca g :=
+      match g with
+      | cut' b1 a => a 
+      | _ => [::]
+      end.
+
+    Definition alt':= (seq G').
+
+    Section add_ca'.
+      Definition add_ca' always alts (a : G') := (*always:= adds always alts to cut *)
+        match a with
+        | cut' lvl a1 => cut' lvl (if always || lvl then a1 ++ alts else a1)
+        | call' pr t => call' pr t
+        end.
+
+      Lemma add_ca1_empty {b lA}:
+        map (add_ca' b [::]) lA = lA.
+      Proof.
+        rewrite /add_ca; elim: lA b => //= x xs IH b.
+        rewrite IH/=; case:x => //= ??; rewrite cats0 if_same//.
+      Qed.
+
+      Lemma map_add1_cas_empty {lA b}:
+        map (map (add_ca' b [::])) lA  = lA.
+      Proof.
+        rewrite /add_ca; elim: lA => //= x xs ->.
+        f_equal; apply add_ca1_empty.
+      Qed.
+    End add_ca'.
+
+    Section incr_cut.
+      Definition incr_cut A :=
+        match A with
+        | cut' _ ca => cut' true ca
+        | _ => A
+        end.
+
+      Definition is_cutb' A := match A with cut' _ _ => true | _ => false end.
+      Definition cuts' A := all is_cutb' A.
+
+
+      Definition incr_cuts := map (map incr_cut).
+
+      Lemma incr_cuts_cat {l1 l2}: incr_cuts (l1 ++ l2) = incr_cuts l1 ++ incr_cuts l2.
+      Proof. rewrite/incr_cuts map_cat//. Qed.
+
+      Lemma incr_cuts0 {l}: incr_cuts l = [::] -> l =[::].
+      Proof. case: l => //. Qed.
+
+      Lemma incr_cut2 {l}: map incr_cut (map incr_cut l) = map incr_cut l.
+      Proof. elim: l => // x xs /=->; case: x => //. Qed.
+
+      Lemma incr_cuts2 {l}: incr_cuts (incr_cuts l) = incr_cuts l.
+      Proof. elim: l => // x xs /=->; rewrite incr_cut2//. Qed.
+
+      Lemma is_cuts_incr_cut {x}:
+        is_cutb' (incr_cut x) = is_cutb' x.
+      Proof. case:x => //. Qed.
+
+      Lemma cuts_incr_cuts {x}:
+        cuts' [seq incr_cut j | j <- x] = cuts' x.
+      Proof. elim: x => //x xs/=<-; rewrite is_cuts_incr_cut//. Qed.
+
+      Lemma cut_add_ca {l b x}: is_cutb' (add_ca' l b x) = is_cutb' x.
+      Proof. case: x => //=*; case:ifP => //. Qed.
+
+      Lemma cuts_add_ca {x l b} : cuts' [seq add_ca' b l j | j <- x] = cuts' x.
+      Proof. elim: x b l => // x xs H/= l b; rewrite H cut_add_ca//. Qed.
+
+      Lemma cuts_cat {x y} : cuts' (x ++ y) = cuts' x && cuts' y.
+      Proof. rewrite/cuts' all_cat//. Qed.
+    End incr_cut.
+
+    Section makers.
+
+      Definition add_deep_help add_deep (n:nat) l :=
+        (apply_cut1 (fun x => map (fun x => x ++ l) ((add_deep n l) x))).
+    
+      Fixpoint add_deep n (l: alt') (A: seq alt') :=
+        match n with
+        | 0 => A
+        | n.+1 =>
+          map (map (add_deep_help add_deep n l)) A
+        end. 
+
+      Definition ad l A := (add_deep (size A) l) A.
+
+      Lemma simpl_ad_cons {n l x xs}:
+        (add_deep n l [:: x & xs]) = add_deep n l [::x] ++ add_deep n l xs.
+      Proof. destruct n => //. Qed.
+
+      Lemma add_deep_empty n l:
+        add_deep n l [:: [::]] = [:: [::]].
+      Proof. destruct n => //. Qed.
+
+      Lemma add_deep_empty1 n l:
+        add_deep n l [::] = [::].
+      Proof. destruct n => //. Qed.
+
+      (* here we add the alts only to deep cut *)
+      Definition make_lB lB tl := map (map (add_ca' false tl)) lB.
+
+      Definition make_lB0 (xs:seq alt') (lB0: alt') := map (fun x => x ++ lB0) xs.
+
+      (* We are build an And node, x and xs are the alternatives from the
+         lhs of the And, lB the alternatives of the rhs and lB0 the reset point.
+         All the cut_to alternatives in x and xs must have lB0 as tail: 
+         this is done thanks to "add (hd x xs)"
+         Moreover, we add to the non superficial cuts in lB the alternatives coming
+         from xs, i.e. in a state (A \/ B) /\_r (! \/ C), the cut should
+         recall (B /\ r) has cut-to alts, in this example, x = A, xs = B, lB0 = r, lB = !; C
+      *)
+      Definition add_alt (x: alt') (xs lB0 lB:list alt') : list  alt' :=
+        match lB0 with
+        (* in a valid state lb0 is either cut away, i.e. has length 0, or
+           is a base_and, i.e. of length 1
+        *)
+        | [::hd] => 
+            (* trully x xs hd lB *)
+            match ad hd (x::xs) with
+            | x::xs =>
+              (* trully x xs hd lB *)
+                let: tl := make_lB0 xs hd in
+                let: lB := make_lB lB tl in
+                [seq x ++ y | y <- lB] ++ tl
+            | [::] => [::]
+            end
+        | [::] =>
+            (* since the reset point is nil, xs are killed (we append the bot to all alt)  *)
+            [seq x ++ y | y <- lB]
+        | _ => [::] (*unreachable*)
+        end.
+
+      Lemma size_lB {lB tl}: size (make_lB lB tl) = size lB.
+      Proof. rewrite size_map//. Qed.
+
+      Lemma size_lB0 {xs hd}: size (make_lB0 xs hd) = size xs.
+      Proof. rewrite size_map//. Qed.
+
+      Lemma size_add_deep n h xs: size xs <= n -> size (add_deep n h xs) = size xs.
+      Proof. elim: n xs => //n IH xs; rewrite size_map//. Qed.
+
+      Lemma size_ad h xs: size (ad h xs) = size xs.
+      Proof. apply: size_add_deep => //. Qed.
+
+      Lemma size_add_alt (x: alt') (xs lB0 lB:list alt') :
+        size (add_alt x xs lB0 lB) <= size (xs ++ lB).
+      Proof. case: lB0 => //=[|y []]//; rewrite !size_cat !size_map addnC//leq_addr//. Qed.
+
+      Lemma make_lB_empty1 {tl} : make_lB [::] tl = [::].
+      Proof. move=>//. Qed.
+
+      Lemma make_lB_empty2 {lB} : make_lB lB [::] = lB.
+      Proof. rewrite/make_lB map_add1_cas_empty//. Qed.
+
+      Lemma make_lB0_empty1 {lb0} : make_lB0 [::] lb0 = [::].
+      Proof. rewrite /make_lB0//. Qed.
+
+      Lemma add_alt_empty3 {x xs lB}:
+        add_alt x xs [::] lB = [seq x ++ y | y <- lB].
+      Proof. rewrite/add_alt//. Qed.
+
+      Lemma add_alt_empty4 {x xs hd}:
+        add_alt x xs [::hd] [::] = behead (make_lB0 (ad hd (x::xs)) hd).
+      Proof. move=>//. Qed.
+    End makers.
+
+    (* bt is the backtracking list for the cut-alternatives
+      this list is important since in this tree:
+           or   
+          /  \  
+         or   K 
+        /  \    
+       !    J   
+      K is in bt but not J, i.e. we have to consider two different levels:
+      the "siblings" on the right of a cut are NOT alternatives
+      the "great^n uncles" on the right of a cut ARE alternatives
+    *)
+    Fixpoint state_to_list_aux (A: state) (bt : list alt') : list alt' :=
+      match A with
+        (* Attenzione: bisogna tradurre: "Dead /\ p" che è diverso da "OK /\ p", quindi è strano
+          Mettere la lista vuota per "OK".
+        *)
+      | OK => [::[::]]
+      | Top => [::[::]]
+      | Bot => [::]
+      | Dead => [::]
+      | Goal _ Cut => [::[::cut' false [::]]]
+      | Goal pr (Call t) => [::[::call' pr t]]
+      | Or A _ B => 
+        let lB := state_to_list_aux B [::] in
+        let lA := state_to_list_aux A lB in
+        (* here we are adding bt to lA. In the example above J in not in bt  *)
+        (* since bt are at least grand-parents alts, then we force the insertion 
+           in the cuts of lA *)
+        incr_cuts (map (map (add_ca' true bt)) (lA ++ lB))
+      | And A B0 B =>
+        let lA   := state_to_list_aux A bt in
+        let lB   := state_to_list_aux B bt in
+        let lB0 := state_to_list_aux B0 bt in
+        if lA is x :: xs then add_alt x xs lB0 lB
+        else [::]
+      end.
+
+    Section size.
+      Fixpoint alternatives A :=
+        match A with
+        | Or A _ B => (alternatives A) + alternatives B
+        | And A B0 B => alternatives A + alternatives B
+        | _ => 1
+        end.
+
+      Lemma size_s2l_leq_alternative A l:
+          size (state_to_list_aux A l) <= alternatives A.
+      Proof.
+        elim: A l => //.
+        - move=> p []//.
+        - move=> A HA s B HB l/=.
+          rewrite !size_map size_cat.
+          have:= HB [::].
+          remember (state_to_list_aux B _) as X eqn:HX.
+          have:= HA X.
+          remember (state_to_list_aux A _) as Y eqn:HY.
+          apply leq_add.
+        - move=> A HA B0 _ B HB l/=.
+          move: (HA l).
+          case X: (state_to_list_aux A l) => [|x xs]//=.
+          have:= (size_add_alt x xs (state_to_list_aux B0 l) (state_to_list_aux B l)).
+          remember (add_alt _ _ _ _) as Z eqn:HZ.
+          move=>/=.
+          rewrite size_cat.
+          have:= HB l.
+          remember (state_to_list_aux B _) as LB.
+          move=> HLB {}HZ Hxs.
+          apply: leq_trans HZ _.
+          apply: leq_add.
+          - by apply: ltnW.
+          - exact: HLB.
+      Qed.
+    End size.
+
+    Section G2G.
+
+      Fixpoint G2G A := 
+        match A with 
+        | call' pr t => call pr t 
+        | cut' _ ca => cut (map (map G2G) ca)
+        end.
+
+      Definition G2Gs l := (map (map G2G) l).
+      Lemma G2Gs_cat l1 l2 : G2Gs (l1 ++ l2) = G2Gs l1 ++ G2Gs l2.
+      Proof. rewrite/G2Gs map_cat//. Qed.
+
+      Definition state_to_list A l := G2Gs (state_to_list_aux A l).
+
+      Lemma G2G_incr_cut {B}: map G2G (map incr_cut B) = map G2G B.
+      Proof. elim: B => //x xs IH/=; rewrite IH; case: x => //. Qed.
+
+      Lemma G2Gs_incr_cuts_cat B C: (G2Gs (incr_cuts B ++ C)) = G2Gs (B ++ C).
+      Proof. elim: B => //x xs H/=; rewrite H G2G_incr_cut//. Qed.
+
+      Lemma G2Gs_incr_cuts {B}: (G2Gs (incr_cuts B)) = G2Gs B.
+      Proof. have:= G2Gs_incr_cuts_cat B [::]; rewrite !cats0//. Qed.
+
+      Lemma G2G_incr_cut_add_ca {hd l}:
+        map G2G (map incr_cut (map (add_ca' true l) hd)) = map (add_ca (G2Gs l)) (map G2G hd).
+      Proof. elim: hd => //=x xs ->;f_equal; case: x => //= _ l1; rewrite map_cat//. Qed.
+    
+    End G2G.
+
+
+    Fixpoint all_tail {T:Type} F (l1 l2:list T) :=
+      match l1 with
+      | [::] => true
+      | x::xs => F x (behead l2) && all_tail F xs (behead l2)
+      end.
+
+    Fixpoint valid_ca_aux n L1 L2 :=
+      match n with
+      | 0 => true
+      | n.+1 =>
+        all_tail (fun xs ys => all (if_cut1 (fun alts => valid_ca_aux n alts alts && suffix (G2Gs alts) (G2Gs ys))) xs) L1 L2
+      end.
+
+    Arguments suffix {T}%_type_scope _ _.
+    Arguments prefix {T}%_type_scope _ _.
+
+
+    Lemma state_to_list_dead {A l}: is_dead A -> state_to_list_aux A l = [::].
+    Proof.
+      elim: A l => //.
+      - move=> A HA s B HB/= l/andP[dA dB]; rewrite HB// HA//.
+      - move=> A HA B0 HB0 B HB l /=dA; rewrite HA//=.
+    Qed.
+
+    Lemma base_and_ko_state_to_list {A l}: base_and_ko A -> state_to_list_aux A l = [::].
+    Proof. elim: A => //=-[]//. Qed.
+
+    Lemma base_or_aux_ko_state_to_list_aux {A l}: base_or_aux_ko A -> state_to_list_aux A l = [::].
+    Proof.
+      elim: A l => //.
+      - move=> /= A HA s B HB l /andP[bA bB]/=; rewrite HB//= base_and_ko_state_to_list//.
+      - move=>[]//.
+    Qed.
+
+    Lemma base_and_state_to_list {A}: base_and A -> exists hd, forall l, state_to_list_aux A l = [::hd].
+    Proof.
+      elim: A => //.
+      - by eexists.
+      - move=> []//p a _ B0 _ B HB/=/andP[/eqP->bB].
+        have [hd H]/= := HB bB.
+        rewrite/state_to_list/=.
+        case: a => [|t]; eexists => l; rewrite H//.
+    Qed.
+
+    Lemma bbAnd_state_to_list {A}:
+      bbAnd A -> 
+        ((forall l, state_to_list_aux A l = [::]) \/ exists hd, forall l, state_to_list_aux A l = [::hd]).
+    Proof.
+      rewrite/bbAnd=>/orP[].
+        move=>/base_and_state_to_list; auto.
+      move=>/base_and_ko_state_to_list; auto.
+    Qed.
+
+
+    Definition points_to1 (l1: seq alt') A := match A with cut' _ l2 => l1 == l2 | _ => true end.
+    Definition empty_ca1 := points_to1 [::].
+    Definition points_to l1 A := match A with cut l2 => l1 == l2 | _ => true end.
+    Definition empty_ca := points_to [::].
+
+
+    Lemma base_and_empty_ca {A B l}:
+      base_and A -> state_to_list_aux A l = B -> all (all empty_ca1) B.
+    Proof.
+      move=> + <-; clear B.
+      elim: A l => //.
+      move=> []// p a _ B0 _ B HB l/=/andP[/eqP->bB].
+      have:= HB l.
+      have [hd H]:= base_and_state_to_list bB; rewrite H.
+      move=>/(_ bB)/=/andP[H1 _].
+      case: a => [|t]//=; rewrite add_ca1_empty H1//.
+    Qed.
+
+    Lemma empty_ca_valid {n hd l}:
+      all empty_ca1 hd -> valid_ca_aux n [::hd] l.
+    Proof.
+      elim: n hd l => //n IH hd l H/=.
+      rewrite andbT.
+      elim: hd H => //=x xs H1 /andP[H2 H3].
+      rewrite H1// andbT.
+      case: x H2 => // _ _/=/eqP<-/=.
+      rewrite suffix0s; destruct n => //.
+    Qed.
+
+
+    Lemma base_and_valid A r n l rs:
+      base_and A ->
+        state_to_list_aux A l = r -> valid_ca_aux n r rs.
+    Proof.
+      move=>H H1; subst.
+      have [hd H2]:= base_and_state_to_list H.
+      have /=/andP[H1 _]:= base_and_empty_ca H (H2 [::]).
+      rewrite H2/=.
+      rewrite empty_ca_valid//.
+    Qed.
+
+    Lemma base_and_ko_valid A r n l rs:
+      base_and_ko A ->
+        state_to_list_aux A l = r -> valid_ca_aux n r rs.
+    Proof. move=>/base_and_ko_state_to_list-><-; destruct n => //. Qed.
+
+    Lemma base_or_aux_ko_valid A r n l rs:
+      base_or_aux_ko A ->
+        state_to_list_aux A l = r -> valid_ca_aux n r rs.
+    Proof. move=>/base_or_aux_ko_state_to_list_aux-><-; destruct n => //. Qed.
+
+
+    Lemma valid_cas1_deep_split_cons x y n l:
+      valid_ca_aux n (x :: y) l =
+        valid_ca_aux n [::x] l && valid_ca_aux n y (behead l).
+    Proof.
+      move=>/=.
+      elim: n y x => //n IH y x/=.
+      f_equal; rewrite andbT//.
+    Qed.
+
+    Lemma success_state_to_list_aux {A m}:
+      valid_state A ->
+      success A ->
+        state_to_list_aux A m = [::] :: (state_to_list_aux (clean_success A) m).
+    Proof.
+      elim: A m => //.
+      - move=> A HA s B HB/= m.
+        case: ifP => [dA vB sB|dA /andP[vA bB] sA].
+          rewrite (state_to_list_dead dA)/=.
+          have:= HB _ vB sB=>->.
+          rewrite (state_to_list_dead dA)//=.
+        have -> //:= HA (state_to_list_aux B [::]) vA sA.
+      - move=> A HA B0 HB0 B HB m /= /and5P[oA vA aB] + + /andP[sA sB].
+        rewrite sA/==> vB bB.
+        have H1 := HA m vA sA.
+        have H2 := HB m vB sB.
+        rewrite HA//HB//.
+        have:= bB; rewrite/bbAnd=>/orP[]{}bB; last first.
+          rewrite (base_and_ko_state_to_list bB)//=.
+        have [hd H3] := base_and_state_to_list bB.
+        rewrite H3//.
+    Qed.
+
+
+    Lemma valid_cas1_empty1 {x l}: valid_ca_aux x [::] l.
+    Proof. destruct x =>//. Qed.
+    
+    Section valid_empty_2_empty_ca.
+      Lemma valid_cas1_empty14 {n gs}:
+        (forall l, size l <= n -> valid_ca_aux n l [::] -> all (all empty_ca1) l) ->
+        (all (if_cut1 (fun alts => valid_ca_aux n alts alts && suffix (G2Gs alts) [::])) gs) -> 
+        all empty_ca1 gs.
+      Proof.
+        move: n.
+        have H := list_induction _ _
+          (fun gs => forall n,
+            (forall l, size l <= n -> valid_ca_aux n l [::] -> all (all empty_ca1) l) ->
+            all (if_cut1 (fun alts => valid_ca_aux n alts alts && suffix (G2Gs alts) [::])) gs ->
+            all empty_ca1 gs).
+        apply: H => //.
+        - move=> /= g Hg {}gs Hgs n H/andP[H1 H2].
+          rewrite (Hgs n)//andbT.
+          destruct g => //=.
+          move: H1 => /=/andP[_].
+          rewrite suffixs0.
+          destruct l => //.
+        - apply: is_list_inhab id _.
+      Qed.
+
+      Lemma valid_cas1_empty13 {n gs}:
+        (forall l : seq (seq G'), size l <= n -> valid_ca_aux n l [::] -> all (all empty_ca1) l) ->
+        size gs < n.+1 ->
+        all_tail (fun gs ys =>
+      all (if_cut1 (fun alts => valid_ca_aux n alts alts && suffix (G2Gs alts) (G2Gs ys))) gs) gs [::] -> 
+      all (all empty_ca1) gs.
+      Proof.
+        move: n.
+        have H := list_induction _ _ 
+          (fun gs => forall n,
+            (forall l, size l <= n -> valid_ca_aux n l [::] -> all (all empty_ca1) l) ->
+          size gs < n.+1 ->
+          all_tail
+            (fun xs0 ys => all (if_cut1 (fun alts => valid_ca_aux n alts alts && suffix (G2Gs alts) (G2Gs ys))) xs0)
+            gs [::] -> all (all empty_ca1) gs).
+        apply: H => //.
+        - move=>/= g Hg {}gs Hgs n H1 H2 /andP[H3 H4].
+          rewrite (Hgs n) => //; last first.
+            apply: ltn_trans (ltnSn _) H2.
+            clear gs Hgs H2 H4.
+          rewrite (@valid_cas1_empty14 n)//.
+        - apply: is_list_inhab id _.
+      Qed.
+
+
+      Lemma valid_cas1_empty2 {n l}: 
+        size l <= n ->
+        valid_ca_aux n l [::] -> all (all (empty_ca1)) l.
+      Proof.
+        elim: n l => //[[]|]// n IH [].
+          move=>//.
+        move=> x xs H; simpl in H.
+        rewrite (valid_cas1_deep_split_cons x xs)//=.
+        move=>/andP[/andP[H1 _] H2].
+        rewrite (@valid_cas1_empty13 n)//andbT.
+        apply: valid_cas1_empty14 IH H1.
+      Qed.
+    End valid_empty_2_empty_ca.
+
+    Section valid_incr_both.
+      Lemma kaka1 n m1 m2 l g:
+        (forall (m3 m4 : nat) (x l : seq (seq G')), size x <= size l ->
+          size l <= n ->
+          valid_ca_aux (n + m3) x l = valid_ca_aux (n + m4) x l) ->  size l <= n ->
+        if_cut1 (fun alts : seq (seq G') => valid_ca_aux (n + m1) alts alts && suffix (G2Gs alts) (G2Gs l)) g =
+        if_cut1 (fun alts : seq (seq G') => valid_ca_aux (n + m2) alts alts && suffix (G2Gs alts) (G2Gs l)) g.
+      Proof.
+        destruct g => //=.
+        move=> H1 H2.
+        case E: suffix; rewrite ?andbF//!andbT.
+        have:= size_suffix E.
+        rewrite !size_map => H.
+          apply: H1 => //.
+          apply: leq_trans H H2.
+      Qed.
+
+      Lemma kaka {n m1 m2} {xs gs}:
+        (forall (m1 m2 : nat) (x l : seq (seq G')),
+          size x <= size l ->
+          size l <= n ->
+          valid_ca_aux (n + m1) x l = valid_ca_aux (n + m2) x l) ->
+          size xs <= n ->
+            all (if_cut1 (fun alts => valid_ca_aux (n + m1) alts alts && suffix (G2Gs alts) (G2Gs xs))) gs =
+            all (if_cut1 (fun alts => valid_ca_aux (n + m2) alts alts && suffix (G2Gs alts) (G2Gs xs))) gs.
+      Proof.
+        move: n m1 m2 xs.
+        have H := list_induction _ _ (fun gs => forall (n m1 m2 : nat) (xs : seq (seq G')),
+          (forall m3 m4 x l, size x <= size l -> size l <= n -> 
+            valid_ca_aux (n + m3) x l = valid_ca_aux (n + m4) x l) ->
+        size xs <= n ->
+        all (if_cut1 (fun alts => valid_ca_aux (n + m1) alts alts && suffix (G2Gs alts) (G2Gs xs))) gs =
+        all (if_cut1 (fun alts => valid_ca_aux (n + m2) alts alts && suffix (G2Gs alts) (G2Gs xs))) gs).
+        apply: H => //.
+        - move=> g Hg {}gs IH n m1 m2 l H1 H2 /=.
+          f_equal; last first.
+            apply: IH H1 H2.
+          apply: kaka1 H1 H2.
+        - apply: is_list_inhab id _.
+      Qed.
+
+      Lemma cricri n m1 m2 gs l:
+        (forall m3 m4 x0 l,
+          size x0 <= size l ->
+          size l <= n ->
+          valid_ca_aux (n + m3) x0 l = valid_ca_aux (n + m4) x0 l) ->
+          size gs < (size l).+1 ->
+        size l < n.+1 ->
+        all_tail (fun xs0 ys => 
+          all (if_cut1 (fun alts => valid_ca_aux (n + m1) alts alts && suffix (G2Gs alts) (G2Gs ys))) xs0) gs l =
+        all_tail (fun xs0 ys => 
+          all (if_cut1 (fun alts => valid_ca_aux (n + m2) alts alts && suffix (G2Gs alts) (G2Gs ys))) xs0) gs l.
+      Proof.
+        move: n m1 m2 l.
+        have H := list_induction _ _ 
+          (fun gs => forall n m1 m2 l,
+            (forall m3 m4 x0 l0,
+              size x0 <= size l0 ->
+              size l0 <= n ->
+              valid_ca_aux (n + m3) x0 l0 = valid_ca_aux (n + m4) x0 l0) ->
+            size gs < (size l).+1 ->
+            size l < n.+1 ->
+            all_tail (fun xs0 ys => all (if_cut1 (fun alts => valid_ca_aux (n + m1) alts alts && suffix (G2Gs alts) (G2Gs ys))) xs0) gs l =
+            all_tail (fun xs0 ys => all (if_cut1 (fun alts => valid_ca_aux (n + m2) alts alts && suffix (G2Gs alts) (G2Gs ys))) xs0) gs l).
+        apply: H => //.
+        - move=> /=g Hg {}gs Hgs n m1 m2 l H1 H2 H3.
+          f_equal; last first.
+            apply: Hgs H1 _ _.
+            destruct l => //.
+            destruct l; simpl in * => //.
+            apply: ltn_trans (ltnSn _) H3.
+          apply: kaka H1 _.
+          destruct l => //=.
+          apply: ltn_trans (ltnSn _) H3.
+        - apply: is_list_inhab id _.
+      Qed.
+
+      Lemma valid_ca_mn {n x l} m1 m2:
+        size x <= size l -> size l <= n ->
+        valid_ca_aux (n+m1) x l = valid_ca_aux (n + m2) x l.
+      Proof.
+        elim: n m1 m2 x l => //[|].
+          move=> ?? []//=.
+            move=> [|x xs]; rewrite ?valid_cas1_empty1//=.
+          move=> ? l1 []//.
+        move=> n Hn m1 m2 [|g gs] l H1 H2.
+          do 2 rewrite valid_cas1_empty1//.
+        simpl in H1.
+        have H3 := ltn_addr _ (ltn_leq_trans _ _ _ H1 H2).
+        do 2 rewrite (valid_cas1_deep_split_cons g gs )//; clear H3.
+        move=>/=.
+        f_equal; [f_equal|].
+          case: l H1 H2 => //=x xs H1 H2.
+          apply: kaka Hn H2.
+        case: l H1 H2 => //=x xs.
+        apply: cricri Hn.
+      Qed.
+    End valid_incr_both.
+
+    Section valid_ca_split_cat.
+
+      Lemma valid_cas1_deep_split_cat_help n xs ys tl:
+        (forall xs ys l,
+          size (xs ++ ys) <= size l ->
+          size l <= n ->
+          valid_ca_aux n (xs ++ ys) l =
+          valid_ca_aux n xs l && valid_ca_aux n ys (drop (size xs) l)) ->
+          size xs + size ys <= (size tl) ->
+          size tl <= n ->
+          valid_ca_aux n.+1 (xs ++ ys) tl =
+          valid_ca_aux n.+1 xs tl &&
+          valid_ca_aux n.+1 ys (drop (size xs) tl).
+      Proof.
+        move: n ys tl.
+        have H := list_induction _ _
+        (fun xs => forall (n : nat) (ys tl : seq (seq G')),
+          (forall xs0 ys0 l : seq (seq G'),
+          size (xs0 ++ ys0) <= size l ->
+          size l <= n ->
+          valid_ca_aux n (xs0 ++ ys0) l =
+          valid_ca_aux n xs0 l &&
+          valid_ca_aux n ys0 (drop (size xs0) l)) ->
+          size xs + size ys <= size tl ->
+          size tl <= n ->
+          valid_ca_aux n.+1 (xs ++ ys) tl =
+          valid_ca_aux n.+1 xs tl &&
+          valid_ca_aux n.+1 ys (drop (size xs) tl)).
+        apply: H => //=.
+        - move=> *; rewrite drop0//.
+        - move=> x Hx {}xs Hxs n ys tl H.
+          rewrite addSn => H1 H2.
+          rewrite -andbA; f_equal.
+          destruct tl => //=.
+          rewrite Hxs//.
+          simpl in H2.
+          apply: ltnW H2.
+        - apply: is_list_inhab id _.
+      Qed.
+
+      Lemma valid_ca_split {x y n l}:
+        size (x++y) <= size l -> size l <= n ->
+        valid_ca_aux n (x ++ y) l =
+          valid_ca_aux n x l && valid_ca_aux n y (drop (size x) l).
+      Proof.
+        move=>/=.
+        elim: n y x l => //n IH y x l.
+        case: x => //[|x xs]; rewrite ?drop0//.
+        rewrite cat_cons; simpl size; rewrite size_cat => H1 H2.
+        rewrite valid_cas1_deep_split_cons//; last first.
+        rewrite (valid_cas1_deep_split_cons x xs)//; last first.
+        rewrite -andbA; f_equal.
+        clear x.
+        destruct l; simpl behead; simpl drop.
+          destruct xs => //.
+        simpl in H1, H2; clear l.
+        rewrite valid_cas1_deep_split_cat_help //.
+        move=> *.
+        apply: IH => //.
+      Qed.
+    End valid_ca_split_cat.
+
+    Lemma valid_ca_incr_cut {n r rs}:
+      valid_ca_aux n (incr_cuts r) rs = valid_ca_aux n r rs.
+    Admitted.
+
+    Section base_valid.
+
+      Lemma base_or_aux_valid A r n rs:
+        base_or_aux A ->
+          state_to_list_aux A [::] = r -> valid_ca_aux n r rs.
+      Proof.
+        move=>+<-; clear r.
+        elim: A n rs => //.
+        - move=>[]//.
+        - move=> A HA s B HB n rs/=/andP[bA bB].
+          rewrite map_add1_cas_empty.
+          have [hd H]:= base_and_state_to_list bA.
+          rewrite H valid_ca_incr_cut/= valid_cas1_deep_split_cons//=.
+          rewrite (HB)//.
+          rewrite empty_ca_valid//.
+          have:=base_and_empty_ca bA (H [::]) => /andP[->]//.
+        - move=> []//p a _ _ _ B HB n rs/=/andP[/eqP->] bB.
+          have [h H]:= base_and_state_to_list bB.
+          rewrite H.
+          have /andP[H1 _]:=base_and_empty_ca bB (H [::]).
+          case: a => [|t] //=; rewrite add_ca1_empty; apply: empty_ca_valid =>//.
+      Qed.
+
+      Lemma bbOr_valid A r rs n:
+        bbOr A ->
+          state_to_list_aux A [::] = r -> valid_ca_aux n r rs.
+      Proof.
+        rewrite/bbOr=>/orP[].
+          apply: base_or_aux_valid.
+        apply: base_or_aux_ko_valid.
+      Qed.
+
+      (* Lemma bbOr_valid1 A r rs n l:
+        bbOr A ->
+          state_to_list_aux A l = r -> valid_ca_aux n r rs.
+      Proof.
+        rewrite/bbOr=>/orP[]; last first.
+          apply: base_or_aux_ko_valid.
+        apply: base_or_aux_valid.
+      Qed. *)
+    End base_valid.
+
+    Lemma split_list_size {T : Type} (x y : nat) (z : seq T) :
+      x + y <= size z ->
+      exists r s : seq T, size r = x /\ r ++ s = z.
+    Proof.
+      move=> Hle.
+      exists (take x z), (drop x z).
+      split; last first.
+      - rewrite cat_take_drop//.
+      - rewrite size_take.
+        have {}Hle: x <= size z.
+          apply: leq_trans (leq_addr _ _) Hle.
+        case: (@eqVneq _ x (size z)).
+          move=>->; rewrite if_same//.
+        move=> H.
+        have:= ltn_neqAle x (size z).
+        rewrite Hle H =>->//.
+    Qed.
+
+    Section valid_make_lb0.
+      Lemma valid_make_lB0_help1 g gs m n ws hd:
+        (forall (m : nat) (l0 ws : seq (seq G')) (hd : seq G'),
+  size l0 <= size ws ->
+  size ws <= n ->
+  size l0 <= m ->
+  valid_ca_aux n l0 ws ->
+  valid_ca_aux n
+    [seq x ++ hd
+       | x <- [seq [seq add_deep_help add_deep m hd j0
+                      | j0 <- j]
+                 | j <- l0]]) ->
+      size ws < n.+1 ->
+all
+    (if_cut1
+       (fun alts : seq (seq G') =>
+        valid_ca_aux n alts alts &&
+        suffix (G2Gs alts) (G2Gs ws)))
+    g ->all
+  (if_cut1
+     (fun alts : seq (seq G') =>
+      valid_ca_aux n alts alts &&
+      suffix (G2Gs alts) (G2Gs ws)))
+  ([seq add_deep_help add_deep m hd j | j <- g] ++ hd).
+(* . *)
+
+      Lemma valid_make_lB0_help l:
+        forall n : nat,
+          (forall (m : nat) (l0 ws : seq (seq G')) (hd : seq G'),
+          size l0 <= size ws ->
+          size ws <= n ->
+          size l0 <= m ->
+          valid_ca_aux n l0 ws ->
+          valid_ca_aux n
+            (make_lB0
+                [seq [seq add_deep_help add_deep m hd k | k <- k]
+                  | k <- l0]
+                hd)
+            ws) ->
+          forall (m : nat) (ws : seq (seq G')) (hd : seq G'),
+          size l <= size ws ->
+          size ws <= n.+1 ->
+          size l <= m ->
+          all_tail
+            (fun (xs : seq G') (ys : seq (seq G')) =>
+            all
+              (if_cut1
+                  (fun alts : seq (seq G') =>
+                  valid_ca_aux n alts alts &&
+                  suffix (G2Gs alts) (G2Gs ys)))
+              xs)
+            l ws ->
+          all_tail
+            (fun (xs : seq G') (ys : seq (seq G')) =>
+            all
+              (if_cut1
+                  (fun alts : seq (seq G') =>
+                  valid_ca_aux n alts alts &&
+                  suffix (G2Gs alts) (G2Gs ys)))
+              xs)
+            (make_lB0
+              [seq [seq add_deep_help add_deep m hd k | k <- k]
+                  | k <- l]
+              hd)
+            ws.
+      Proof.
+        have H := list_induction _ _
+        (fun l => forall n : nat,
+(forall (m : nat) (l0 ws : seq (seq G')) (hd : seq G'),
+ size l0 <= size ws ->
+ size ws <= n ->
+ size l0 <= m ->
+ valid_ca_aux n l0 ws ->
+ valid_ca_aux n
+   (make_lB0
+      [seq [seq add_deep_help add_deep m hd j | j <- j]
+         | j <- l0]
+      hd)
+   ws) ->
+forall (m : nat) (ws : seq (seq G')) (hd : seq G'),
+size l <= size ws ->
+size ws <= n.+1 ->
+size l <= m ->
+all_tail
+  (fun (xs : seq G') (ys : seq (seq G')) =>
+   all
+     (if_cut1
+        (fun alts : seq (seq G') =>
+         valid_ca_aux n alts alts &&
+         suffix (G2Gs alts) (G2Gs ys)))
+     xs)
+  l ws ->
+all_tail
+  (fun (xs : seq G') (ys : seq (seq G')) =>
+   all
+     (if_cut1
+        (fun alts : seq (seq G') =>
+         valid_ca_aux n alts alts &&
+         suffix (G2Gs alts) (G2Gs ys)))
+     xs)
+  (make_lB0
+     [seq [seq add_deep_help add_deep m hd j | j <- j]
+        | j <- l]
+     hd)
+  ws).
+        apply: H => //.
+        - rewrite/make_lB0.
+          move=> /=g Hg gs Hgs n H m []//=w ws hd H1 H2 H3/andP[H4 H5].
+          rewrite Hgs//; last first; try by by apply ltnW.
+          rewrite andbT.
+          clear gs Hgs H1 H3 H5.
+
+        
+
+      Lemma valid_make_lB0 {n m l ws hd}:
+        size l <= size ws -> size ws <= n -> size l <= m ->
+        valid_ca_aux n l ws -> 
+        valid_ca_aux n (make_lB0 (map (map (add_deep_help add_deep m hd)) l) hd) ws.
+      Proof.
+        elim: n m l ws hd => //= + + + l. n IH m l ws hd H1 H2 H3 H4.
+        rewrite/make_lB0.
+        move: 
+        destruct hd => //=.
+          rewrite /add_deep_help.
+          rewrite cats0.
+
+      Admitted.
+    End valid_make_lb0.
+
+    (* Lemma state_to_list_clean_success_size: *)
+      
+
+
+    Lemma ttt A r rs n l:
+        valid_state A -> state_to_list_aux A l = r -> 
+          size r <= size rs -> size rs <= n -> valid_ca_aux n r rs.
+    Proof.
+      move=> + <-; clear r.
+      elim: A n l rs => //; try by move=>[].
+      - move=> p/= [|t]/= n l rs _ _ _; apply empty_ca_valid => //.
+      - move=> A HA s B HB n l rs/=.
+        case:ifP => [dA vB|dA /andP[vA bB]]; rewrite !size_map.
+          rewrite size_cat map_cat.
+          rewrite state_to_list_dead//= valid_ca_incr_cut=> H1 H2.
+          (have: l = [::] by admit); move=>?; subst.
+          rewrite map_add1_cas_empty.
+          apply: HB vB H1 H2.
+        rewrite valid_ca_incr_cut map_cat size_cat.
+        (have: l = [::] by admit); move=>?; subst.
+        rewrite 2!map_add1_cas_empty => H1 H2.
+        rewrite valid_ca_split ?size_cat//.
+        rewrite (HA)//=; last first.
+          apply: leq_trans (leq_addr _ _) H1.
+        have [l1[l2[H3 H4]]]:= split_list_size _ _ _ H1; subst.
+        rewrite -H3 drop_size_cat//.
+        rewrite -H3 size_cat leq_add2l in H1.
+        rewrite size_cat in H2.
+        apply: HB (VS.bbOr_valid bB) H1 _.
+        apply: leq_trans (leq_addl _ _) H2.
+      - move=> A HA B0 _ B HB n l rs/=/and5P[oA vA aB].
+        case:ifP => /=[sA vB bB0|sA/eqP->].
+          rewrite success_state_to_list_aux//.
+          have [H|[hd H]] := bbAnd_state_to_list bB0.
+            rewrite H/= map_id.
+            apply: HB vB.
+          rewrite H/=map_id size_cat size_lB size_lB0 size_map.
+          move=> H1 H2.
+          rewrite valid_ca_split//; last first.
+            rewrite size_cat size_lB size_lB0 size_map//.
+          apply/andP; split; last first.
+            rewrite size_lB.
+            have [w[ws [H3?]]]:= split_list_size _ _ _ H1; subst.
+            rewrite -H3 size_cat leq_add2l in H1.
+            rewrite size_cat in H2.
+            rewrite -H3.
+            rewrite drop_size_cat//.
+            have H4 : size ws < n.+1.
+              apply: leq_trans (leq_addr _ _) _.
+              rewrite addSn addnC.
+              apply H2.
+            have:= HA n.+1 l ([::] :: ws) vA _ H4.
+            rewrite success_state_to_list_aux//.
+            move=>/(_ H1).
+            rewrite valid_cas1_deep_split_cons.
+            move=>/andP[_]; simpl behead.
+            rewrite -addn1.
+            rewrite (valid_ca_mn _ 0)//addn0.
+            rewrite/make_lB0.
+            apply: valid_make_lB0 => //.
+            .
+
+
+
+
+          
+          rewrite size_cat size_.
+          (have: l = [::] by admit); move=>?; subst.
+          rewrite 
+
+    Admitted.
+
+    (* Lemma ratatata {l1 n l2 m}:
+      size l2 < n -> size l2 < m ->
+      (* -> valid_ca_aux n l2 -> *)
+      map (add_deep_help add_deep n l1) l2 =
+      map (add_deep_help add_deep m l1) l2.
+    Proof.
+      have H := list_induction _ 
+        (fun g => forall n l1, add_deep_help add_deep n.+1 l1 g = add_deep_help add_deep n l1 g)
+        (fun l2 => forall n l1, 
+          map (add_deep_help add_deep n.+1 l1) l2 = map (add_deep_help add_deep n l1) l2).
+      apply: H => //.
+      - clear l1 n l2 => g Hg gs IH n l1/=.
+        rewrite IH; f_equal.
+        apply: Hg.
+      - apply: is_list_inhab.
+        rewrite/full.
+        destruct g => /=.
+
+      rewrite/add_deep_help.
+      move=>/=.
+    Admitted.
+
+    Lemma ratatata1 {x bs}:
+      [seq [seq add_deep_help add_deep (size bs).+1 x j | j <- j] | j <- bs] =
+      [seq [seq add_deep_help add_deep (size bs) x j | j <- j] | j <- bs].
+    Admitted. *)
+
+End Nur.
+
